
Now we need to apply the [chain rule](math-prereqs.qmd#thm-chain-rule):

$$
\blue{\deriv{\beta}\logf{1+\exp{\vx_i'\beta}}} =
\red{\deriv{\beta}\cb{1+\exp{\vx_i'\beta}}} \frac{1}{1+\exp{\vx_i'\beta}}
$$

$$
\ba
\red{\deriv{\beta}\cb{1+\exp{\vx_i'\beta}}}
&= \deriv{\beta}\exp{\vx_i'\beta}
\\ &= \paren{\deriv{\beta}\vx_i'\beta} \exp{\vx_i'\beta}
\\ &= \vx_i \exp{\vx_i'\beta}
\\ &= \red{\vx_i \omega_i}
\ea
$${#eq-deriv-expit}

So:

$$
\ba
\blue{\deriv{\beta}\logf{1+\exp{\vx_i'\beta}}}
   &= \red{\vx_i \omega_i} \frac{1}{1+\exp{\vx_i'\beta}}
\\ &= \frac{\red{\vx_i \omega_i}}{1+\exp{\vx_i'\beta}}  \vx_i
\\ &= \vx_i \expitf{\vx_i'\beta}
\\ &= \blue{\vx_i \pi_i}
\ea
$$
