
Then:

$$\beta_{0} = \eta(P=0,A=0)$${#eq-wcgs-intxn-beta0}

$$
\ba
\beta_A
&= \deriv{a}\eta(P=0, A = a)
\\&= \eta(P = 0, A = a + 1)- \eta(P = 0, A = a)
\ea
$${#eq-wcgs-intxn-betaA}

$$\b_P = \eta(P = 1, A = 0) - \eta(P=0, A = 0)$${#eq-wcgs-intxn-betaP}

$$
\ba
\beta_{PA}
&= \deriv{a}\eta(P=1, A = a) - \deriv{a}\eta(P=0, A = a)
\\
&= \sb{\eta(1,a + 1)- \eta(1, a)} -
\sb{\eta(0,a + 1)- \eta(0, a)}
\\
&= \sb{\eta(1,a + 1)- \eta(0,a + 1)} -
\sb{\eta(1, a)- \eta(0, a)}
\ea
$${#eq-wcgs-intxn-betaPA}
