::: proof

Using @lem-deriv-invodds:

$$
\ba
\dexpitf{\logodds}
   &= \deriv{\logodds} \expitf{\logodds}
\\ &= \deriv{\logodds} \invoddsf{\expf{\logodds}}
\\ &= \dinvoddsf{\expf{\logodds}}  \deriv{\logodds}\expf{\logodds}
\\ &=  \frac{1}{\sqf{1 + \expf{\logodds}}} \expf{\logodds}
\\ &=  \frac{\expf{\logodds}}{\sqf{1 + \expf{\logodds}}}
\\ &=  \frac{\expf{\logodds}}{1 + \expf{\logodds}} \frac{1}{1 + \expf{\logodds}}
\\ &=  \expitf{\logodds} (1-\expitf{\logodds})
\ea
$$

Alternatively, we can use @thm-expit:

$$
\ba
\dexpitf{\logodds}
   &= \deriv{\logodds} \expitf{\logodds}
\\ &= \deriv{\logodds} (1 + \exp{-\logodds})^{-1}
\\ &= -(1 + \exp{-\logodds})^{-2} \deriv{\logodds} (1 + \exp{-\logodds})
\\ &= -(1 + \exp{-\logodds})^{-2} (-\exp{-\logodds})
\\ &= (1 + \exp{-\logodds})^{-2} (\exp{-\logodds})
\\ &= (1 + \exp{-\logodds})^{-1} \frac{\exp{-\logodds}}{1 + \exp{-\logodds}}
\\ &= (1 + \exp{-\logodds})^{-1} \frac{1}{1 + \exp{\logodds}}
\\ &= \expitf{\logodds} (1-\expitf{\logodds})
\ea
$$
:::
