{{< include macros.qmd >}}

If $(a^b)^c = a^{(b^c)}$, then since $(a^b)^c = a^{bc}$,
we have:
$$a^{bc} = a^{(b^c)}$$
$$\logf{a^{bc}} = \logf{a^{(b^c)}}$$
$$bc \cdot \logf{a} = b^c\cdot \logf{a}$${#eq-double-exp-log-scale}

@eq-double-exp-log-scale holds in each of the following cases:

1. $bc = b^c$ (see @exr-exp-vs-mult).
2. $a=1$ (i.e., $\logf{a} = 0$).
3. $a=0$ (i.e., $\logf{a}= -\infty$) 
*and* $\signf{bc}=\signf{b^c}$.

In particular, when $a=0$ and $c=0$,
$bc = 0$ and $b^c = 1$ (for any $b \in \mathbb{R}$),
so $\signf{bc}\neq \signf{b^c}$, and
$(a^b)^c \neq a^{(b^c)}$:

$$
\ba
(a^b)^c
&= (0^b)^0
\\
&= 1
\ea
$$

$$
\ba
a^{(b^c)}
&= 0^{(b^0)}
\\
&= 0^1
\\
&= 0
\ea
$$

