
:::{#thm-deriv-polynomial}
#### Derivatives of polynomials

$$\deriv{x}x^q = qx^{q-1}$$

:::

---

:::{#thm-deriv-log}

#### derivative of natural logarithm
$$\dlogf{x} = \frac{1}{x} = x^{-1}$$
:::

:::{#thm-deriv-exp}
#### derivative of exponential
$$\dexpf{x} = \expf{x}$$
:::

---

:::{#thm-product-rule}
#### Product rule
$$(ab)' = ab' + ba'$$
:::

:::{#thm-quotient-rule}
#### Quotient rule
$$(a/b)' = a'/b - (a/b^2)b'$$
:::

:::{#thm-chain-rule}
#### Chain rule
$$\derivf{a}{c} = \derivf{a}{b} \derivf{b}{c}$$

i.e., 

$$(f(g(x))' = f'(g(x)) g'(x)$$
:::

---

:::{#cor-deriv-log-chain}

#### Chain rule for logarithms
$$
\deriv{x}\log{f(x)} = \frac{f'(x)}{f(x)}
$$

:::

::: proof
Apply @thm-chain-rule and @thm-deriv-log.
:::

---
